eval/work/isabelle-lwe-regev-01/LatticeCrypto.thy
@@ -21,6 +21,13 @@ record lwe_ciphertext =
   ct_u :: int_vec
   ct_v :: int
 
+(* Dimension safety predicates *)
+definition valid_matrix :: "int_matrix => nat => nat => bool" where
+  "valid_matrix A m n = (length A = m \<and> (\<forall>row \<in> set A. length row = n))"
+
+definition valid_vec :: "int_vec => nat => bool" where
+  "valid_vec v n = (length v = n)"
+
 definition vec_add :: "int_vec => int_vec => int_vec" where
   "vec_add xs ys = map2 (+) xs ys"
 
@@ -35,6 +42,17 @@ definition mat_vec_mult :: "int_matrix => int_vec => int_vec" where
 
 definition mat_transpose_vec_mult :: "int_matrix => int_vec => int_vec" where
   "mat_transpose_vec_mult A r = mat_vec_mult (transpose A) r"
+
+(* Length preservation lemmas *)
+lemma vec_add_length:
+  "length v1 = length v2 \<Longrightarrow> length (vec_add v1 v2) = length v1"
+  unfolding vec_add_def by simp
+
+lemma vec_mod_length: "length (vec_mod v q) = length v"
+  unfolding vec_mod_def by simp
+
+lemma mat_vec_mult_length: "length (mat_vec_mult A x) = length A"
+  unfolding mat_vec_mult_def by simp
 
 lemma inner_prod_vec_add:
   assumes len_xy: "length x = length y"
@@ -57,7 +75,8 @@ definition encode_bit :: "int => bool => int" where
   "encode_bit q b = (if b then q div 2 else 0)"
 
 definition decode_bit :: "int => int => bool" where
-  "decode_bit q d = (d >= q div 2)"
+  "decode_bit q d = (let d' = d mod q in
+    (if d' > q div 2 then q - d' else d') > q div 4)"
 
 lemma div2_pos:
   fixes q :: int
@@ -70,20 +89,109 @@ proof -
   then show ?thesis by simp
 qed
 
+lemma div4_pos:
+  fixes q :: int
+  assumes "q > 4"
+  shows "q div 4 > 0"
+proof -
+  have "4 <= q" using assms by arith
+  have "0 < q div 4"
+    using pos_imp_zdiv_pos_iff[of 4 q] `4 <= q` by simp
+  then show ?thesis by simp
+qed
+
 lemma encode_decode_inverse:
   fixes q :: int
   assumes "q > 2"
   shows "decode_bit q (encode_bit q b) = b"
 proof (cases b)
   case True
+  have q_pos: "q > 0" using assms by arith
+  have half_pos: "q div 2 > 0" using div2_pos[OF assms] .
+  have half_lt_q: "q div 2 < q" using q_pos by simp
+  have mod_half: "(q div 2) mod q = q div 2"
+    using half_pos half_lt_q by simp
+  have not_gt: "\<not> (q div 2 > q div 2)" by simp
+  have quarter_lt_half: "q div 4 < q div 2"
+    using assms by (simp add: zdiv_mono2)
   then show ?thesis
-    by (simp add: decode_bit_def encode_bit_def)
+    using True mod_half not_gt
+    by (simp add: decode_bit_def encode_bit_def Let_def)
 next
   case False
-  have "q div 2 > 0" using div2_pos[OF assms] .
+  have q_pos: "q > 0" using assms by arith
+  have q_nonneg: "q >= 0" using q_pos by arith
+  have zero_mod: "(0::int) mod q = 0" using q_pos by simp
+  (* decode_bit q 0: d' = 0 mod q = 0; 0 > q/2? No; distance = 0; 0 > q/4? No *)
+  have "decode_bit q 0 = False"
+    unfolding decode_bit_def Let_def
+    using q_nonneg by simp
   then show ?thesis
-    using False by (simp add: decode_bit_def encode_bit_def)
+    using False by (simp add: encode_bit_def)
 qed
+
+(* Modular arithmetic helpers *)
+lemma mod_add_cong:
+  fixes q :: int assumes "q > 0"
+  shows "(a mod q + b mod q) mod q = (a + b) mod q"
+  using assms by (simp add: mod_add_eq)
+
+lemma inner_prod_mod_cong:
+  fixes q :: int
+  assumes "q > 0" "length v = length w"
+  shows "inner_prod (vec_mod v q) w mod q = inner_prod v w mod q"
+using assms(2)
+proof (induct v w rule: list_induct2)
+  case Nil
+  then show ?case by (simp add: inner_prod_def vec_mod_def)
+next
+  case (Cons x xs y ys)
+  have "inner_prod (vec_mod (x # xs) q) (y # ys) =
+        (x mod q) * y + inner_prod (vec_mod xs q) ys"
+    by (simp add: inner_prod_def vec_mod_def)
+  also have "... mod q = ((x mod q) * y mod q + inner_prod (vec_mod xs q) ys mod q) mod q"
+    using assms(1) by (simp add: mod_add_eq)
+  also have "... = ((x mod q) * y mod q + inner_prod xs ys mod q) mod q"
+    using Cons by simp
+  also have "... = ((x * y) mod q + inner_prod xs ys mod q) mod q"
+    using assms(1) by (metis mod_mult_left_eq)
+  also have "... = (x * y + inner_prod xs ys) mod q"
+    using assms(1) by (simp add: mod_add_eq)
+  also have "... = inner_prod (x # xs) (y # ys) mod q"
+    by (simp add: inner_prod_def)
+  finally show ?case .
+qed
+
+lemma inner_prod_mod_cong_right:
+  fixes q :: int
+  assumes "q > 0" "length v = length w"
+  shows "inner_prod v (vec_mod w q) mod q = inner_prod v w mod q"
+using assms(2)
+proof (induct v w rule: list_induct2)
+  case Nil
+  then show ?case by (simp add: inner_prod_def vec_mod_def)
+next
+  case (Cons x xs y ys)
+  have "inner_prod (x # xs) (vec_mod (y # ys) q) =
+        x * (y mod q) + inner_prod xs (vec_mod ys q)"
+    by (simp add: inner_prod_def vec_mod_def)
+  also have "... mod q = (x * (y mod q) mod q + inner_prod xs (vec_mod ys q) mod q) mod q"
+    using assms(1) by (simp add: mod_add_eq)
+  also have "... = (x * (y mod q) mod q + inner_prod xs ys mod q) mod q"
+    using Cons by simp
+  also have "... = ((x * y) mod q + inner_prod xs ys mod q) mod q"
+    using assms(1) by (metis mod_mult_right_eq)
+  also have "... = (x * y + inner_prod xs ys) mod q"
+    using assms(1) by (simp add: mod_add_eq)
+  also have "... = inner_prod (x # xs) (y # ys) mod q"
+    by (simp add: inner_prod_def)
+  finally show ?case .
+qed
+
+(* Note: The inner product transpose identity <s, A^T r> = <As, r> is a standard
+   linear algebra fact. In this formalization, we assume it via the iprod assumption
+   in the main lemmas, as the full proof requires careful matrix dimension tracking
+   that would distract from the cryptographic correctness focus. *)
 
 definition lwe_encrypt :: "lwe_public_key => int => int_vec => bool => lwe_ciphertext" where
   "lwe_encrypt pk q r m =
@@ -98,96 +206,259 @@ definition lwe_decrypt :: "lwe_secret_key => int => lwe_ciphertext => bool" wher
 
 lemma decryption_error_term:
   fixes q :: int
-  assumes b_def: "pk_b pk = vec_add (mat_vec_mult (pk_A pk) (sk_s sk)) e"
+  assumes q_pos: "q > 0"
+    and b_def: "pk_b pk = vec_mod (vec_add (mat_vec_mult (pk_A pk) (sk_s sk)) e) q"
     and len_e: "length (mat_vec_mult (pk_A pk) (sk_s sk)) = length e"
     and len_r: "length r = length (mat_vec_mult (pk_A pk) (sk_s sk))"
-    and u_bound: "vec_mod (mat_transpose_vec_mult (pk_A pk) r) q =
-                  mat_transpose_vec_mult (pk_A pk) r"
-    and v_bound: "(inner_prod (pk_b pk) r + encode_bit q m) mod q =
-                  inner_prod (pk_b pk) r + encode_bit q m"
+    and len_b: "length (pk_b pk) = length r"
+    and len_sk: "length (mat_transpose_vec_mult (pk_A pk) r) = length (sk_s sk)"
     and iprod: "inner_prod (sk_s sk) (mat_transpose_vec_mult (pk_A pk) r) =
                 inner_prod (mat_vec_mult (pk_A pk) (sk_s sk)) r"
   shows "(ct_v (lwe_encrypt pk q r m) -
           inner_prod (sk_s sk) (ct_u (lwe_encrypt pk q r m))) mod q =
          (inner_prod e r + encode_bit q m) mod q"
 proof -
-  have b_iprod:
-    "inner_prod (pk_b pk) r =
-     inner_prod (mat_vec_mult (pk_A pk) (sk_s sk)) r + inner_prod e r"
+  let ?As = "mat_vec_mult (pk_A pk) (sk_s sk)"
+  have len_add: "length (vec_add ?As e) = length ?As"
+    using len_e by (simp add: vec_add_length)
+  have b_iprod_mod:
+    "inner_prod (pk_b pk) r mod q =
+     (inner_prod ?As r + inner_prod e r) mod q"
   proof -
-    have "inner_prod (pk_b pk) r =
-          inner_prod (vec_add (mat_vec_mult (pk_A pk) (sk_s sk)) e) r"
+    have "inner_prod (pk_b pk) r mod q =
+          inner_prod (vec_mod (vec_add ?As e) q) r mod q"
       using b_def by simp
-    also have "... =
-          inner_prod (mat_vec_mult (pk_A pk) (sk_s sk)) r + inner_prod e r"
+    also have "... = inner_prod (vec_add ?As e) r mod q"
+      using inner_prod_mod_cong[OF q_pos] len_add len_r
+      by (simp add: vec_mod_length)
+    also have "... = (inner_prod ?As r + inner_prod e r) mod q"
       using len_e len_r by (simp add: inner_prod_vec_add)
     finally show ?thesis .
   qed
-  have u_ct:
-    "ct_u (lwe_encrypt pk q r m) = mat_transpose_vec_mult (pk_A pk) r"
-    using u_bound by (simp add: lwe_encrypt_def)
-  have v_ct:
-    "ct_v (lwe_encrypt pk q r m) = inner_prod (pk_b pk) r + encode_bit q m"
-    using v_bound by (simp add: lwe_encrypt_def)
-  show ?thesis
-    using b_iprod u_ct v_ct iprod
+  have u_ct: "ct_u (lwe_encrypt pk q r m) = vec_mod (mat_transpose_vec_mult (pk_A pk) r) q"
+    by (simp add: lwe_encrypt_def)
+  have v_ct: "ct_v (lwe_encrypt pk q r m) = (inner_prod (pk_b pk) r + encode_bit q m) mod q"
+    by (simp add: lwe_encrypt_def)
+  have u_iprod: "inner_prod (sk_s sk) (ct_u (lwe_encrypt pk q r m)) mod q =
+                 inner_prod (sk_s sk) (mat_transpose_vec_mult (pk_A pk) r) mod q"
+  proof -
+    have "inner_prod (sk_s sk) (ct_u (lwe_encrypt pk q r m)) mod q =
+          inner_prod (sk_s sk) (vec_mod (mat_transpose_vec_mult (pk_A pk) r) q) mod q"
+      using u_ct by simp
+    also have "... = inner_prod (sk_s sk) (mat_transpose_vec_mult (pk_A pk) r) mod q"
+      using inner_prod_mod_cong_right[OF q_pos] len_sk
+      by (simp add: vec_mod_length)
+    finally show ?thesis .
+  qed
+  (* Now show the main result *)
+  let ?As_r = "inner_prod ?As r"
+  have sk_u_eq: "inner_prod (sk_s sk) (ct_u (lwe_encrypt pk q r m)) mod q = ?As_r mod q"
+    using u_iprod iprod by simp
+  have step1: "(ct_v (lwe_encrypt pk q r m) - inner_prod (sk_s sk) (ct_u (lwe_encrypt pk q r m))) mod q =
+        ((inner_prod (pk_b pk) r + encode_bit q m) mod q - inner_prod (sk_s sk) (ct_u (lwe_encrypt pk q r m))) mod q"
+    using v_ct by simp
+  (* Use the fact that (a mod q - b) mod q = (a - b) mod q *)
+  have mod_sub: "\<And>a b. (a mod q - b) mod q = (a - b) mod q"
+    using q_pos by (simp add: mod_diff_left_eq)
+  have step2: "((inner_prod (pk_b pk) r + encode_bit q m) mod q - inner_prod (sk_s sk) (ct_u (lwe_encrypt pk q r m))) mod q =
+        (inner_prod (pk_b pk) r + encode_bit q m - inner_prod (sk_s sk) (ct_u (lwe_encrypt pk q r m))) mod q"
+    using mod_sub by simp
+  have step3: "(inner_prod (pk_b pk) r + encode_bit q m - inner_prod (sk_s sk) (ct_u (lwe_encrypt pk q r m))) mod q =
+        (inner_prod (pk_b pk) r - inner_prod (sk_s sk) (ct_u (lwe_encrypt pk q r m)) + encode_bit q m) mod q"
     by (simp add: algebra_simps)
+  (* Use modular congruence: a mod q = b mod q implies (a - b) mod q = 0 *)
+  have b_mod: "inner_prod (pk_b pk) r mod q = (?As_r + inner_prod e r) mod q"
+    using b_iprod_mod by simp
+  have u_mod: "inner_prod (sk_s sk) (ct_u (lwe_encrypt pk q r m)) mod q = ?As_r mod q"
+    using sk_u_eq by simp
+  (* The key computation - direct calculation *)
+  have step4: "(inner_prod (pk_b pk) r - inner_prod (sk_s sk) (ct_u (lwe_encrypt pk q r m)) + encode_bit q m) mod q =
+               (inner_prod e r + encode_bit q m) mod q"
+  proof -
+    let ?b_r = "inner_prod (pk_b pk) r"
+    let ?sk_u = "inner_prod (sk_s sk) (ct_u (lwe_encrypt pk q r m))"
+    have eq1: "(?b_r - ?sk_u) mod q = (?b_r mod q - ?sk_u mod q) mod q"
+      using q_pos by (simp add: mod_diff_eq)
+    have eq2: "?b_r mod q - ?sk_u mod q = (?As_r + inner_prod e r) mod q - ?As_r mod q"
+      using b_mod u_mod by simp
+    have eq3: "((?As_r + inner_prod e r) mod q - ?As_r mod q) mod q = (?As_r + inner_prod e r - ?As_r) mod q"
+      using q_pos by (simp add: mod_diff_eq)
+    have eq4: "?As_r + inner_prod e r - ?As_r = inner_prod e r"
+      by simp
+    have diff_mod: "(?b_r - ?sk_u) mod q = inner_prod e r mod q"
+      using eq1 eq2 eq3 eq4 by simp
+    have "(?b_r - ?sk_u + encode_bit q m) mod q = ((?b_r - ?sk_u) mod q + encode_bit q m mod q) mod q"
+      using q_pos by (simp add: mod_add_eq)
+    also have "... = (inner_prod e r mod q + encode_bit q m mod q) mod q"
+      using diff_mod by simp
+    also have "... = (inner_prod e r + encode_bit q m) mod q"
+      using q_pos by (simp add: mod_add_eq)
+    finally show ?thesis .
+  qed
+  show ?thesis using step1 step2 step3 step4 by simp
 qed
 
 lemma correctness_condition:
   fixes q :: int
-  assumes q_gt: "q > 2"
-    and b_def: "pk_b pk = vec_add (mat_vec_mult (pk_A pk) (sk_s sk)) e"
+  assumes q_gt: "q > 4"
+    and b_def: "pk_b pk = vec_mod (vec_add (mat_vec_mult (pk_A pk) (sk_s sk)) e) q"
     and len_e: "length (mat_vec_mult (pk_A pk) (sk_s sk)) = length e"
     and len_r: "length r = length (mat_vec_mult (pk_A pk) (sk_s sk))"
-    and u_bound: "vec_mod (mat_transpose_vec_mult (pk_A pk) r) q =
-                  mat_transpose_vec_mult (pk_A pk) r"
-    and v_bound: "(inner_prod (pk_b pk) r + encode_bit q m) mod q =
-                  inner_prod (pk_b pk) r + encode_bit q m"
+    and len_b: "length (pk_b pk) = length r"
+    and len_sk: "length (mat_transpose_vec_mult (pk_A pk) r) = length (sk_s sk)"
     and iprod: "inner_prod (sk_s sk) (mat_transpose_vec_mult (pk_A pk) r) =
                 inner_prod (mat_vec_mult (pk_A pk) (sk_s sk)) r"
-    and noise_mod: "(inner_prod e r + encode_bit q m) mod q =
-                    inner_prod e r + encode_bit q m"
-    and noise_abs: "abs (inner_prod e r) < q div 4"
-    and noise_nonneg: "0 <= inner_prod e r"
+    and error_bound: "\<bar>inner_prod e r\<bar> < q div 4"
   shows "lwe_decrypt sk q (lwe_encrypt pk q r m) = m"
-proof (cases m)
-  case False
+proof -
+  have q_pos: "q > 0" using q_gt by arith
+  let ?noise = "inner_prod e r"
   have d_eq:
+    "(ct_v (lwe_encrypt pk q r m) -
+      inner_prod (sk_s sk) (ct_u (lwe_encrypt pk q r m))) mod q =
+     (?noise + encode_bit q m) mod q"
+    using decryption_error_term[OF q_pos b_def len_e len_r len_b len_sk iprod] .
+  have decrypt_eq:
     "lwe_decrypt sk q (lwe_encrypt pk q r m) =
-      decode_bit q ((inner_prod e r + encode_bit q m) mod q)"
-    using decryption_error_term[OF b_def len_e len_r u_bound v_bound iprod]
-    by (simp add: lwe_decrypt_def)
-  have d_eq2:
-    "decode_bit q ((inner_prod e r + encode_bit q m) mod q) =
-     decode_bit q (inner_prod e r)"
-    using False noise_mod by (simp add: encode_bit_def)
-  have q_nonneg: "0 <= q" using q_gt by arith
-  have div4_le: "q div 4 <= q div 2"
-    using zdiv_mono2[of q 4 2] q_nonneg by simp
-  have noise_lt4: "inner_prod e r < q div 4"
-    using noise_abs noise_nonneg by simp
-  have noise_lt2: "inner_prod e r < q div 2"
-    using noise_lt4 div4_le by arith
-  have "decode_bit q (inner_prod e r) = False"
-    using noise_lt2 by (simp add: decode_bit_def)
-  then show ?thesis
-    using d_eq d_eq2 False by simp
-next
-  case True
-  have d_eq:
-    "lwe_decrypt sk q (lwe_encrypt pk q r m) =
-      decode_bit q ((inner_prod e r + encode_bit q m) mod q)"
-    using decryption_error_term[OF b_def len_e len_r u_bound v_bound iprod]
-    by (simp add: lwe_decrypt_def)
-  have d_eq2:
-    "decode_bit q ((inner_prod e r + encode_bit q m) mod q) =
-     decode_bit q (inner_prod e r + q div 2)"
-    using True noise_mod by (simp add: encode_bit_def)
-  have "decode_bit q (inner_prod e r + q div 2) = True"
-    using noise_nonneg by (simp add: decode_bit_def)
-  then show ?thesis
-    using d_eq d_eq2 True by simp
+     decode_bit q ((?noise + encode_bit q m) mod q)"
+    using d_eq by (simp add: lwe_decrypt_def)
+  show ?thesis
+  proof (cases m)
+    case False
+    (* m = False, so encode_bit q m = 0 *)
+    have enc_false: "encode_bit q False = 0" by (simp add: encode_bit_def)
+    have noise_val: "(?noise + encode_bit q m) mod q = ?noise mod q"
+      using False enc_false by simp
+    (* With |noise| < q/4, the distance from 0 is |noise|, which is < q/4 *)
+    (* So decode_bit returns False (distance <= q/4) *)
+    have noise_small: "\<bar>?noise\<bar> < q div 4" using error_bound .
+    (* noise mod q: if noise in [0, q/4), stays as is; if noise in (-q/4, 0), becomes q+noise *)
+    have "decode_bit q (?noise mod q) = False"
+    proof -
+      let ?d' = "?noise mod q"
+      have q_gt2: "q > 2" using q_gt by arith
+      have q_div4_pos: "q div 4 > 0" using div4_pos[OF q_gt] .
+      have q_div2_pos: "q div 2 > 0" using div2_pos[OF q_gt2] .
+      (* Case analysis on sign of noise *)
+      show ?thesis
+      proof (cases "?noise >= 0")
+        case True
+        (* noise in [0, q/4), so noise mod q = noise *)
+        have "?noise < q div 4" using noise_small True by simp
+        hence "?noise < q" using q_gt by simp
+        hence d'_eq: "?d' = ?noise" using True by simp
+        (* d' = noise < q/4 < q/2, so not > q/2 *)
+        have "\<not> (?d' > q div 2)" using d'_eq `?noise < q div 4` q_div4_pos by simp
+        (* distance = d' = noise < q/4 *)
+        hence "decode_bit q ?d' = (?d' > q div 4)"
+          by (simp add: decode_bit_def Let_def)
+        thus ?thesis using d'_eq `?noise < q div 4` True by simp
+      next
+        case False
+        (* noise in (-q/4, 0), so noise mod q = q + noise *)
+        have noise_neg: "?noise < 0" using False by simp
+        have noise_gt: "?noise > - (q div 4)" using noise_small by simp
+        have noise_gt_neg_q: "?noise > -q" using noise_gt q_gt by simp
+        (* For -q < a < 0 and q > 0: a mod q = a + q *)
+        have d'_eq: "?d' = q + ?noise"
+        proof -
+          have "?noise + q >= 0" using noise_gt_neg_q by simp
+          have "?noise + q < q" using noise_neg by simp
+          thus ?thesis using `?noise + q >= 0` `?noise + q < q` q_pos
+            by (metis add.commute mod_add_self2 mod_pos_pos_trivial)
+        qed
+        (* q + noise > q - q/4 = 3q/4 > q/2 *)
+        have "q + ?noise > q - q div 4" using noise_gt by simp
+        have "q - q div 4 >= q div 2" using q_gt by simp
+        hence d'_gt: "?d' > q div 2" using `q + ?noise > q - q div 4` d'_eq by simp
+        (* distance = q - d' = q - (q + noise) = -noise < q/4 *)
+        have dist_eq: "q - ?d' = - ?noise" using d'_eq by simp
+        have dist_lt: "- ?noise < q div 4" using noise_small noise_neg by simp
+        have "decode_bit q ?d' = (q - ?d' > q div 4)"
+          using d'_gt by (simp add: decode_bit_def Let_def)
+        thus ?thesis using dist_eq dist_lt by simp
+      qed
+    qed
+    thus ?thesis using decrypt_eq noise_val False by simp
+  next
+    case True
+    (* m = True, so encode_bit q m = q div 2 *)
+    have enc_true: "encode_bit q True = q div 2" by (simp add: encode_bit_def)
+    have val: "(?noise + encode_bit q m) mod q = (?noise + q div 2) mod q"
+      using True enc_true by simp
+    have noise_small: "\<bar>?noise\<bar> < q div 4" using error_bound .
+    (* noise + q/2 should decode to True (distance from q/2 is |noise| < q/4) *)
+    have "decode_bit q ((?noise + q div 2) mod q) = True"
+    proof -
+      let ?sum = "?noise + q div 2"
+      have q_gt2: "q > 2" using q_gt by arith
+      have q_div4_pos: "q div 4 > 0" using div4_pos[OF q_gt] .
+      have q_div2_pos: "q div 2 > 0" using div2_pos[OF q_gt2] .
+      (* sum is in (q/2 - q/4, q/2 + q/4) = (q/4, 3q/4) *)
+      have sum_lb: "?sum > q div 4"
+        using noise_small q_div2_pos by simp
+      have sum_ub: "?sum < q div 2 + q div 4"
+        using noise_small by simp
+      have sum_lt_q: "?sum < q"
+        using sum_ub q_gt by simp
+      show ?thesis
+      proof (cases "?noise >= 0")
+        case True
+        (* sum in [q/2, 3q/4), stays as is mod q *)
+        have sum_nonneg: "?sum >= 0" using True q_div2_pos by simp
+        have d'_eq: "?sum mod q = ?sum" using sum_nonneg sum_lt_q by simp
+        (* sum <= q/2 + noise < q/2 + q/4 *)
+        have not_gt: "\<not> (?sum > q div 2)" if "?noise = 0"
+          using that by simp
+        (* For noise in [0, q/4): sum in [q/2, 3q/4)
+           If sum <= q/2: distance = sum, need sum > q/4 (yes, since sum >= q/2 > q/4)
+           If sum > q/2: distance = q - sum, need q - sum > q/4
+             q - sum > q - (q/2 + q/4) = q/4 - only if sum < 3q/4 *)
+        show ?thesis
+        proof (cases "?sum > q div 2")
+          case True
+          have dist: "q - ?sum > q div 4"
+            using sum_ub q_gt by simp
+          have "decode_bit q ?sum = (q - ?sum > q div 4)"
+            using True d'_eq by (simp add: decode_bit_def Let_def)
+          thus ?thesis using dist d'_eq by simp
+        next
+          case False
+          (* sum <= q/2 and noise >= 0, so noise + q/2 <= q/2, hence noise <= 0 *)
+          (* Combined with noise >= 0, we get noise = 0, hence sum = q/2 *)
+          have noise_le: "?noise <= 0" using False by simp
+          have noise_eq: "?noise = 0" using True noise_le by simp
+          have sum_eq: "?sum = q div 2" using noise_eq by simp
+          (* decode_bit q (q/2): d' = (q/2) mod q = q/2, not > q/2, so distance = q/2 > q/4 *)
+          have d'_is_half: "?sum mod q = q div 2" using d'_eq sum_eq by simp
+          have not_gt_half: "\<not> (q div 2 > q div 2)" by simp
+          have half_gt_quarter: "q div 2 > q div 4" using q_div2_pos q_div4_pos q_gt by simp
+          (* decode_bit uses d mod q internally, so decode_bit q (d mod q) = decode_bit q d *)
+          have decode_mod: "decode_bit q (?sum mod q) = decode_bit q ?sum"
+            unfolding decode_bit_def by (simp add: mod_mod_trivial)
+          have "decode_bit q ?sum = True"
+            unfolding decode_bit_def Let_def using d'_is_half not_gt_half half_gt_quarter by simp
+          thus ?thesis using decode_mod by simp
+        qed
+      next
+        case False
+        (* noise < 0, so sum in (q/4, q/2) *)
+        have noise_neg: "?noise < 0" using False by simp
+        have sum_lt_half: "?sum < q div 2" using noise_neg by simp
+        have sum_pos: "?sum > 0" using sum_lb q_div4_pos by simp
+        have d'_eq: "?sum mod q = ?sum" using sum_pos sum_lt_q by simp
+        (* sum in (q/4, q/2), so not > q/2, distance = sum > q/4 *)
+        have not_gt: "\<not> (?sum > q div 2)" using sum_lt_half by simp
+        have decode_mod: "decode_bit q (?sum mod q) = decode_bit q ?sum"
+          unfolding decode_bit_def by (simp add: mod_mod_trivial)
+        have "decode_bit q ?sum = (?sum > q div 4)"
+          using not_gt d'_eq by (simp add: decode_bit_def Let_def)
+        hence "decode_bit q ?sum = True" using sum_lb by simp
+        thus ?thesis using decode_mod by simp
+      qed
+    qed
+    thus ?thesis using decrypt_eq val True by simp
+  qed
 qed
 
 export_code
